main/hl/terse/lean/HL.lean
@@ -5,4 +5,4 @@ import HL.Equiv
 import HL.Hoare
 import HL.Hoare2
 
--- Built on 2026-09-15 00:46 UTC
+-- Built on 2026-09-10 14:28 UTC
