main/hl/terse/lean/HL/Slang.lean
@@ -416,4 +416,4 @@ end Slang.AevalRExtended
 --  Functional: computation. Relational: expressive. Best:
 --  both, proved equivalent.
 
--- Built on 2026-09-15 00:46 UTC
+-- Built on 2026-09-10 14:28 UTC
