main/lf/student/lean/LF/IndProp.lean
@@ -1588,4 +1588,4 @@ theorem pigeonhole_principle {α : Type} {l₁ l₂ : List α}
     Repeats l₁ := by
   sorry
 
--- Built on 2026-09-15 00:44 UTC
+-- Built on 2026-09-10 14:27 UTC
