main/lf/student/lean/LF/Lists.lean
@@ -1232,4 +1232,4 @@ end PartialMap
 
 end Lists
 
--- Built on 2026-09-15 00:44 UTC
+-- Built on 2026-09-10 14:27 UTC
