main/ts/student/lean/TS/StlcProp.lean
@@ -1200,4 +1200,4 @@ theorem progress (t : Tm) (T : Ty) (hT : <{ ∅ ⊢ ~t ⦂ ~T }>) :
 
 end StlcArith
 
--- Built on 2026-09-15 00:46 UTC
+-- Built on 2026-09-10 14:29 UTC
